initial commit

CanonicalForms/Basic.lean
@@ -1,1 +1,85 @@
-def hello := "world"
+import Mathlib.Data.Set.Basic
+import Mathlib.Data.Set.Function
+import Mathlib.Data.Set.Lattice
+import Mathlib.Data.Setoid.Basic
+import Mathlib.Logic.Function.Basic
+import Mathlib.Tactic
+
+namespace CanonicalForms
+
+variable {α β γ : Type*}
+
+def IsInvariant
+    (r : α → α → Prop)
+    (f : α → β) :
+    Prop :=
+  ∀x y : α, r x y → f x = f y
+
+def IsCompleteInvariant
+    (r : α → α → Prop)
+    (f : α → β) :
+    Prop :=
+  ∀x y : α, r x y ↔ f x = f y
+
+theorem IsCompleteInvariant.toIsInvariant
+    (r : α → α → Prop)
+    (f : α → β)
+    (hf : IsCompleteInvariant r f) :
+    IsInvariant r f := by
+  intro x y hxy
+  exact (hf x y).mp hxy
+
+theorem quotientMap_isCompleteInvariant
+    [s : Setoid α] :
+    IsCompleteInvariant (· ≈ ·) (Quotient.mk s) := by
+  intro x y
+  constructor
+  · exact Quotient.sound
+  · exact Quotient.exact
+
+def IsRetractionSectionPair
+    (r : α → β)
+    (s : β → α) :
+    Prop :=
+  r ∘ s = id
+
+theorem IsRetractionSectionPair.pointwise
+    (r : α → β)
+    (s : β → α)
+    (h : IsRetractionSectionPair r s) :
+    ∀ y : β, r (s y) = y := by
+  intro y
+  exact congr_fun h y
+
+theorem IsRetractionSectionPair.section_injective
+    (r : α → β)
+    (s : β → α)
+    (h : IsRetractionSectionPair r s) :
+    Function.Injective s := by
+  intro y₁ y₂ heq
+  have := congr_arg r heq
+  simp [h.pointwise r s] at this
+  exact this
+
+theorem corestriction_surjective_completeInvariant
+    (r : α → α → Prop)
+    (I : α → β)
+    (hI : IsCompleteInvariant r I) :
+    let I' : α → Set.range I := fun x => ⟨I x, Set.mem_range_self x⟩
+    Function.Surjective I' ∧ IsCompleteInvariant r I' := by
+  simp only
+  constructor
+  · intro ⟨y, x, hx⟩
+    exact ⟨x, by simp [hx]⟩
+  · intro x y
+    simp
+    exact hI x y
+
+def corestriction (I : α → β) : α → Set.range I :=
+  fun x => ⟨I x, Set.mem_range_self x⟩
+
+def canonicalFormOfCompleteInvariant
+    (I : α → β)
+    (s' : Set.range I → α) :
+    α → α :=
+  s' ∘ corestriction I
