CanonicalForms/CanonicalForm.lean
@@ -1,0 +1,134 @@
+import Mathlib.Data.Set.Basic
+import Mathlib.Data.Set.Function
+import Mathlib.Data.Set.Lattice
+import Mathlib.Data.Setoid.Basic
+import Mathlib.Logic.Function.Basic
+import Mathlib.Tactic
+
+import CanonicalForms.Basic
+
+namespace CanonicalForms
+
+variable {α β γ : Type*}
+
+structure IsCanonicalForm (r : α → α → Prop) (C : α → α) : Prop where
+  inv    : IsInvariant r C
+  equiv  : ∀x : α, r x (C x)
+
+def skeleton (C : α → α) : Set α := Set.range C
+
+theorem canonicalForm_idempotent (r : α → α → Prop) (C : α → α) (hC : IsCanonicalForm r C) : C ∘ C = C := by
+  funext x
+  exact (hC.inv x (C x) (hC.equiv x)).symm
+
+theorem canonicalForm_to_section [s : Setoid α]
+    (C : α → α)
+    (hC : IsCanonicalForm (· ≈ ·) C) :
+    ∃ sec : Quotient s → α, IsRetractionSectionPair (Quotient.mk s) sec ∧ C = sec ∘ Quotient.mk s := by
+  use Quotient.lift C (fun x y hxy => hC.inv x y hxy)
+  refine ⟨?_section, ?_factoring⟩
+  · funext q
+    induction q using Quotient.ind with
+    | _ x =>
+      simp [Function.comp]
+      rw [← Quotient.sound]
+      exact hC.equiv x
+  · funext x
+    simp [Function.comp]
+
+theorem section_to_canonicalForm [s : Setoid α]
+    (C : α → α)
+    (sec : Quotient s → α)
+    (hpair : IsRetractionSectionPair (Quotient.mk s) sec)
+    (hfact : C = sec ∘ Quotient.mk s) :
+    IsCanonicalForm (· ≈ ·) C := by
+  refine ⟨?_inv, ?_equiv⟩
+  · intro x y hxy
+    simp [hfact]
+    exact congr_arg sec (Quotient.sound hxy)
+  · intro x
+    simp only [IsRetractionSectionPair] at hpair
+    rw [hfact]
+    exact Quotient.exact (congr_fun hpair ⟦x⟧).symm
+
+theorem canonicalForm_iff_section [s : Setoid α]
+    (C : α → α) :
+    IsCanonicalForm (· ≈ ·) C ↔ ∃ sec : Quotient s → α, IsRetractionSectionPair (Quotient.mk s) sec ∧ C = sec ∘ Quotient.mk s := by
+  constructor
+  · exact canonicalForm_to_section C
+  · rintro ⟨sec, hpair, hfact⟩
+    exact section_to_canonicalForm C sec hpair hfact
+
+theorem canonicalForm_iff_section_of_completeInvariant [s : Setoid α]
+  (I : α → β)
+  (hInv : IsCompleteInvariant (· ≈ ·) I)
+  (hSurj : Function.Surjective I)
+  (C : α → α) :
+  IsCanonicalForm (· ≈ ·) C ↔ ∃ sec' : β → α, IsRetractionSectionPair I sec' ∧ C = sec' ∘ I := by
+  rw [canonicalForm_iff_section]
+  have hInv' : IsInvariant (· ≈ ·) I := hInv.toIsInvariant
+  let Ibar : Quotient s → β :=
+    Quotient.lift I (fun x y hxy => hInv' x y hxy)
+  have hIbar_inj : Function.Injective Ibar := by
+    intro q₁ q₂ heq
+    induction q₁ using Quotient.ind with
+    | _ x =>
+      induction q₂ using Quotient.ind with
+      | _ y =>
+      simp [Ibar] at heq
+      exact Quotient.sound ((hInv x y).mpr heq)
+  have hIbar_surj : Function.Surjective Ibar := by
+    intro b
+    obtain ⟨x, hx⟩ := hSurj b
+    exact ⟨Quotient.mk s x, hx⟩
+  have hIbar_bij : Function.Bijective Ibar := ⟨hIbar_inj, hIbar_surj⟩
+  let hIbar_inv : β → Quotient s := Function.surjInv hIbar_surj
+  have hIpair : I = Ibar ∘ Quotient.mk s := by
+    funext x
+    exact Eq.symm Function.comp_apply
+  constructor
+  · intro hCan
+    obtain ⟨sec, hpair, hfact⟩ := hCan
+    let sec' : β → α := sec ∘ hIbar_inv
+    have hpair' : IsRetractionSectionPair I sec' := by
+      funext x
+      rw [hIpair]
+      simp only [sec']
+      change (Ibar ∘ (Quotient.mk s ∘ sec) ∘ hIbar_inv) x = id x
+      simp only [IsRetractionSectionPair] at hpair
+      rw [hpair]
+      rw [Function.id_comp]
+      simp only [hIbar_inv]
+      exact Function.surjInv_eq hIbar_surj x
+    have hCpair' : C = sec' ∘ I := by
+      funext x
+      simp only [sec']
+      rw [hfact]
+      simp
+      congr
+      simp only [hIpair]
+      change ⟦x⟧ = (hIbar_inv ∘ Ibar) ⟦x⟧
+      simp only [hIbar_inv]
+      exact (Function.leftInverse_surjInv hIbar_bij ⟦x⟧).symm
+    exact ⟨sec', hpair', hCpair'⟩
+  · intro hCan'
+    obtain ⟨sec', hpair', hfact'⟩ := hCan'
+    let sec : Quotient s → α := sec' ∘ Ibar
+    have hpair : IsRetractionSectionPair (Quotient.mk s) sec := by
+      funext y
+      simp only [sec]
+      induction y using Quotient.ind with
+      | _ x =>
+        change (Quotient.mk s ∘ sec' ∘ Ibar ∘ Quotient.mk s) x = ⟦x⟧
+        rw [← hIpair, ← hfact']
+        simp
+        apply Quotient.sound
+        apply (hInv (C x) x).mpr
+        simp only [hfact', Function.comp]
+        simp only [IsRetractionSectionPair] at hpair'
+        exact congr_fun hpair' (I x)
+    have hCpair : C = sec ∘ Quotient.mk s := by
+      simp only [sec]
+      rw [Function.comp_assoc, ← hIpair]
+      exact hfact'
+    exact ⟨sec, hpair, hCpair⟩
