CanonicalForms/Existence.lean
@@ -1,0 +1,44 @@
+import Mathlib.Data.Set.Basic
+import Mathlib.Data.Set.Function
+import Mathlib.Data.Set.Lattice
+import Mathlib.Data.Setoid.Basic
+import Mathlib.Logic.Function.Basic
+import Mathlib.Tactic
+
+import CanonicalForms.Basic
+import CanonicalForms.CanonicalForm
+
+namespace CanonicalForms
+
+variable {α β : Type*}
+
+theorem surjective_has_section
+    (f : α → β)
+    (hf : Function.Surjective f) :
+    ∃ g : β → α, IsRetractionSectionPair f g := by
+  use fun y => Classical.choose (hf y)
+  funext y
+  exact Classical.choose_spec (hf y)
+
+theorem canonicalForm_exists
+    [s : Setoid α] :
+    ∃ C : α → α, IsCanonicalForm (· ≈ ·) C := by
+  have hq_surj : Function.Surjective (Quotient.mk s) := Quotient.mk_surjective
+  obtain ⟨sec, hsec⟩ := surjective_has_section (Quotient.mk s) hq_surj
+  have hC : IsCanonicalForm (· ≈ ·) (sec ∘ Quotient.mk s) := section_to_canonicalForm (sec ∘ Quotient.mk s) sec hsec rfl
+  exact ⟨sec ∘ Quotient.mk s, hC⟩
+
+
+theorem canonicalFormOfCompleteInvariant_exists
+    [s : Setoid α]
+    (I : α → α)
+    (hI : IsCompleteInvariant (· ≈ ·) I) :
+    ∃ C : α → α, ∃ sec' : Set.range I → α, C = canonicalFormOfCompleteInvariant  I sec' ∧ IsCanonicalForm (· ≈ ·) C := by
+  let I' := corestriction I
+  simp only [canonicalFormOfCompleteInvariant]
+  change ∃ C sec', C = sec' ∘ I' ∧ IsCanonicalForm (fun x1 x2 => x1 ≈ x2) C
+  obtain ⟨C, hC⟩ := @canonicalForm_exists α s
+  have hI' : IsCompleteInvariant (· ≈ ·) I' := (corestriction_surjective_completeInvariant s.r I hI).2
+  have hI'_surj : Function.Surjective I' := (corestriction_surjective_completeInvariant s.r I hI).1
+  obtain ⟨sec', hpair', hCpair'⟩ := (canonicalForm_iff_section_of_completeInvariant I' hI' hI'_surj C).mp hC
+  exact ⟨C, sec', hCpair', hC⟩
